mlanguage is its most general shape

theories/mlanguage/mlanguage.v
@@ -4,81 +4,40 @@ From iris.prelude Require Import options.
 From melocoton Require Export multirelations commons.
 
 Section mlanguage_mixin.
-  Context {expr val func ectx state : Type}.
-  Notation mixin_expr_class := (@mixin_expr_class val).
+  Context {expr val func state cont : Type}.
 
-  Context (of_class : mixin_expr_class → expr).
-  Context (to_class : expr → option mixin_expr_class).
+  Context (of_val : val → expr).
+  Context (to_val : expr → option val).
 
-  Context (empty_ectx : ectx).
-  Context (comp_ectx : ectx → ectx → ectx).
-  Context (fill : ectx → expr → expr).
+  Context (is_call : expr → string → list val → cont → Prop).
+  Context (resume_with : cont → expr → expr).
 
   (** A program is a map from function names to function bodies. *)
   Local Notation mixin_prog := (gmap string func).
 
   Context (apply_func : func → list val → option expr).
-  Context (expr_size : expr → nat).
-  Context (head_step : mixin_prog → umrel (expr * state)).
-
-  Notation is_head_redex p x := (head_step p x (λ _, True)).
-  Notation to_val e := (match to_class e with Some (ExprVal v) => Some v | _ => None end).
+  Context (prim_step : mixin_prog → umrel (expr * state)).
 
   Record MlanguageMixin := {
-    (** Expression classification *)
-    mixin_to_of_class c : to_class (of_class c) = Some c;
-    mixin_of_to_class e c : to_class e = Some c → of_class c = e;
+    (** Expression and values *)
+    mixin_to_of_val c : to_val (of_val c) = Some c;
+    mixin_of_to_val e c : to_val e = Some c → of_val c = e;
 
     (** Reduction behavior of the special classes of expressions *)
-    (** mixin_val_head_step is not an iff because the backward direction is trivial *)
-    mixin_val_head_step p v σ X :
-      head_step p (of_class (ExprVal v), σ) X → False;
-    mixin_call_head_step p f vs σ X :
-      head_step p (of_class (ExprCall f vs), σ) X ↔
-      (∀ (fn : func) (e2 : expr),
-        p !! f = Some fn → Some e2 = apply_func fn vs → X (e2, σ));
+    (** mixin_val_prim_step is not an iff because the backward direction is trivial *)
+    mixin_val_prim_step p v σ X :
+      prim_step p (of_val v, σ) X → False;
+    mixin_call_prim_step p e f vs C σ X :
+      is_call e f vs C →
+        prim_step p (e, σ) X ↔
+        (∀ (fn : func) (e2 : expr),
+          p !! f = Some fn → Some e2 = apply_func fn vs → X (resume_with C e2, σ));
 
-    (** Evaluation contexts *)
-    mixin_fill_empty e : fill empty_ectx e = e;
-    mixin_fill_comp K1 K2 e : fill K1 (fill K2 e) = fill (comp_ectx K1 K2) e;
-    mixin_fill_inj K : Inj (=) (=) (fill K);
-    (* The the things in a class contain only values in redex positions (or the
-       redex is the topmost one). *)
-    mixin_fill_class K e :
-      is_Some (to_class (fill K e)) → K = empty_ectx ∨ ∃ v, to_class e = Some (ExprVal v);
-    mixin_fill_size K e :
-      K ≠ empty_ectx → expr_size e < expr_size (fill K e);
-    mixin_call_in_ctx K K' e f vs :
-      fill K e = fill K' (of_class (ExprCall f vs)) →
-      (∃ K'', K' = comp_ectx K K'') ∨ (∃ v, of_class (ExprVal v) = e);
+    mixin_not_is_call e : is_Some (to_val e) ↔ (∀ f vs C, ¬ is_call e f vs C);
 
-    (** Given a head redex [e1_redex] somewhere in a term, and another
-        decomposition of the same term into [fill K' e1'] such that [e1'] is not
-        a value, then the head redex context is [e1']'s context [K'] filled with
-        another context [K''].  In particular, this implies [e1 = fill K''
-        e1_redex] by [fill_inj], i.e., [e1]' contains the head redex.)
-
-        This implies there can be only one head redex, see
-        [head_redex_unique]. *)
-    mixin_step_by_val p K' K_redex e1' e1_redex σ :
-      fill K' e1' = fill K_redex e1_redex →
-      match to_class e1' with Some (ExprVal _) => False | _ => True end →
-      is_head_redex p (e1_redex, σ) →
-      ∃ K'', K_redex = comp_ectx K' K'';
-
-    (** If [fill K e] takes a head step, then either [e] is a value or [K] is
-        the empty evaluation context. In other words, if [e] is not a value
-        wrapping it in a context does not add new head redex positions. *)
-    mixin_head_ctx_step_val p K e σ :
-      is_head_redex p (fill K e, σ) → K = empty_ectx ∨ ∃ v, to_class e = Some (ExprVal v);
-
-    (** If e is not head_reducible, we can recurse into it to find a head_redex in a context.
-        Since context are strictly decreasing, this implies there is no NB (except for values) *)
-    mixin_head_redex_cases p e σ : 
-      is_Some (to_val e)
-    ∨ is_head_redex p (e, σ)
-    ∨ (¬ is_head_redex p (e, σ) ∧
-        (∃ K e', e = fill K e' ∧ to_val e' = None ∧ K ≠ empty_ectx))
+    mixin_prim_step_total p e σ :
+      to_val e = None →
+      prim_step p (e, σ) (λ _, True)
   }.
 End mlanguage_mixin.
 
@@ -88,57 +47,35 @@ Global Notation mixin_prog func := (gmap string func).
 Structure mlanguage {val : Type} := Mlanguage {
   expr : Type;
   func : Type;
-  ectx : Type;
   state : Type;
+  cont : Type;
 
-  of_class : mixin_expr_class val → expr;
-  to_class : expr → option (mixin_expr_class val);
-  empty_ectx : ectx;
-  comp_ectx : ectx → ectx → ectx;
-  fill : ectx → expr → expr;
+  of_val : val → expr;
+  to_val : expr → option val;
+
+  is_call : expr → string → list val → cont → Prop;
+  resume_with : cont → expr → expr;
+
   apply_func : func → list val → option expr;
-  expr_size : expr → nat;
-  head_step : mixin_prog func → umrel (expr * state);
+  prim_step : (gmap string func) → umrel (expr * state);
+
 
   mlanguage_mixin :
-    MlanguageMixin (val:=val) of_class to_class empty_ectx comp_ectx fill
-      apply_func expr_size head_step
+    MlanguageMixin (val:=val) of_val to_val is_call resume_with apply_func prim_step
 }.
 
 Declare Scope expr_scope.
 Bind Scope expr_scope with expr.
 
 Arguments mlanguage : clear implicits.
-Arguments Mlanguage {_ expr _ _ _ _ _ _ _ _ apply_func _ head_step}.
-Arguments of_class {_} _ _.
-Arguments to_class {_ _} _.
-Arguments empty_ectx {_ _}.
-Arguments comp_ectx {_ _} _ _.
-Arguments fill {_ _} _ _.
+Arguments Mlanguage {_ expr _ _ _ _ _ _ resume_with apply_func prim_step}.
+Arguments of_val {_} _ _.
+Arguments to_val {_ _} _.
+Arguments is_call {_ _}.
 Arguments apply_func {_ _}.
-Arguments expr_size {_ _} _.
-Arguments head_step {_ _} _.
-
-Definition expr_class {val} (Λ : mlanguage val) := mixin_expr_class val.
-(* A [Definition] throws off Coq's "old" ("tactic") unification engine *)
+Arguments resume_with {_ _}.
+Arguments prim_step {_ _}.
 Notation prog Λ := (mixin_prog Λ.(func)).
-
-Definition to_val {val} {Λ : mlanguage val} (e : expr Λ) :=
-  match to_class e with
-  | Some (ExprVal v) => Some v
-  | _ => None
-  end.
-Definition of_val {val} (Λ : mlanguage val) (v : val) := of_class Λ (ExprVal v).
-
-Definition to_call {val} {Λ : mlanguage val} (e : expr Λ) :=
-  match to_class e with
-  | Some (ExprCall f v) => Some (f, v)
-  | _ => None
-  end.
-Definition of_call {val} (Λ : mlanguage val) f (v : list val) := of_class Λ (ExprCall f v).
-
-Definition is_head_redex {val} {Λ : mlanguage val} (p : prog Λ) x := head_step p x (λ _, True).
-
 (* From an ectx_language, we can construct a mlanguage. *)
 Section mlanguage.
   Context {val : Type}.
@@ -147,367 +84,48 @@ Section mlanguage.
   Implicit Types v : val.
   Implicit Types vs : list val.
   Implicit Types e : expr Λ.
-  Implicit Types c : expr_class Λ.
-  Implicit Types K : ectx Λ.
+  Implicit Types K : cont Λ.
   Implicit Types p : prog Λ.
   Implicit Types X : expr Λ * state Λ → Prop.
 
-  Lemma to_of_class c : to_class (of_class Λ c) = Some c.
+  Lemma to_of_val c : to_val (of_val Λ c) = Some c.
   Proof. apply mlanguage_mixin. Qed.
-  Lemma of_to_class e c : to_class e = Some c → of_class Λ c = e.
+  Lemma of_to_val e c : to_val e = Some c → of_val Λ c = e.
   Proof. apply mlanguage_mixin. Qed.
 
-  Lemma of_class_inj k1 k2 : of_class Λ k1 = of_class Λ k2 → k1 = k2.
+  Lemma of_val_inj k1 k2 : of_val Λ k1 = of_val Λ k2 → k1 = k2.
   Proof.
     intros H. enough (Some k1 = Some k2) by congruence.
-    rewrite <- !to_of_class. rewrite H. done.
+    rewrite <- !to_of_val. rewrite H. done.
   Qed.
-
-  Lemma to_val_of_call f vs : to_val (of_call Λ f vs) = None.
-  Proof. rewrite /to_val /of_call to_of_class. done. Qed.
-  Lemma to_call_of_val v : to_call (of_val Λ v) = None.
-  Proof. rewrite /to_call /of_val to_of_class. done. Qed.
-  Lemma is_val_is_class e : is_Some (to_val e) → is_Some (to_class e).
-  Proof. rewrite /to_val /is_Some. destruct (to_class e) as [[|]|]; naive_solver. Qed.
-  Lemma is_call_is_class e : is_Some (to_call e) → is_Some (to_class e).
-  Proof. rewrite /to_call /is_Some. destruct (to_class e) as [[|]|]; naive_solver. Qed.
-
-  Lemma val_head_step p v σ X :
-    head_step p (of_class Λ (ExprVal v), σ) X → False.
-  Proof. apply mlanguage_mixin. Qed.
-  Lemma call_head_step p f vs σ X :
-    head_step p (of_class Λ (ExprCall f vs), σ) X ↔
-    (∀ fn e2, p !! f = Some fn → Some e2 = apply_func fn vs → X (e2, σ)).
-  Proof. apply mlanguage_mixin. Qed.
-
-  Lemma fill_empty e : fill empty_ectx e = e.
-  Proof. apply mlanguage_mixin. Qed.
-  Lemma fill_comp K1 K2 e : fill K1 (fill K2 e) = fill (comp_ectx K1 K2) e.
-  Proof. apply mlanguage_mixin. Qed.
-  Global Instance fill_inj K : Inj (=) (=) (fill K).
-  Proof. apply mlanguage_mixin. Qed.
-  Lemma fill_class' K e :
-    is_Some (to_class (fill K e)) → K = empty_ectx ∨ ∃ v, to_class e = Some (ExprVal v).
-  Proof. apply mlanguage_mixin. Qed.
-  Lemma fill_size K e :
-      K ≠ empty_ectx → expr_size e < expr_size (fill K e).
-  Proof. apply mlanguage_mixin. Qed.
-  Lemma step_by_val' p K' K_redex e1' e1_redex σ :
-      fill K' e1' = fill K_redex e1_redex →
-      match to_class e1' with Some (ExprVal _) => False | _ => True end →
-      is_head_redex p (e1_redex, σ) →
-      ∃ K'', K_redex = comp_ectx K' K''.
-  Proof. apply mlanguage_mixin. Qed.
-  Lemma head_ctx_step_val' p K e σ :
-    is_head_redex p (fill K e, σ) → K = empty_ectx ∨ ∃ v, to_class e = Some (ExprVal v).
-  Proof. apply mlanguage_mixin. Qed.
-  Lemma call_in_ctx K K' e f vs :
-    fill K e = fill K' (of_class Λ (ExprCall f vs)) →
-    (∃ K'', K' = comp_ectx K K'') ∨ (∃ v, of_class Λ (ExprVal v) = e).
-  Proof. apply mlanguage_mixin. Qed.
-  Lemma call_in_ctx_to_val K K' e f vs :
-    fill K e = fill K' (of_class _ (ExprCall f vs)) →
-    (∃ K'', K' = comp_ectx K K'') ∨ is_Some (to_val e).
-  Proof.
-    intros [H1|(x&Hx)]%call_in_ctx; auto.
-    right. exists x. rewrite /to_val -Hx to_of_class//.
-  Qed.
-  Lemma head_redex_cases p e σ :
-      is_Some (to_val e)
-    ∨ is_head_redex p (e, σ)
-    ∨ (¬ is_head_redex p (e, σ) ∧
-        (∃ K e', e = fill K e' ∧ to_val e' = None ∧ K ≠ empty_ectx)).
-  Proof. apply mlanguage_mixin. Qed.
-  Lemma fill_class K e :
-    is_Some (to_class (fill K e)) → K = empty_ectx ∨ is_Some (to_val e).
-  Proof.
-    intros [?|[v Hv]]%fill_class'; first by left. right.
-    rewrite /to_val Hv. eauto.
-  Qed.
-  Lemma to_val_fill_call K f vs :
-    to_val (fill K (of_call Λ f vs)) = None.
-  Proof.
-    destruct (to_val (fill K (of_call Λ f vs))) eqn:HH; eauto.
-    destruct (fill_class K (of_call Λ f vs)) as [H1|H2].
-    { unfold to_val in HH. repeat case_match; simplify_eq. eauto. }
-    { subst. rewrite fill_empty in HH. unfold to_val in HH.
-      repeat case_match; simplify_eq.
-      unfold of_call in *. by rewrite -> to_of_class in *. }
-    { clear HH. rewrite -> to_val_of_call in H2. by apply is_Some_None in H2. }
-  Qed.
-  Lemma call_call_in_ctx K K' fn fn' vs vs' :
-    fill K (of_class _ (ExprCall fn vs)) = fill K' (of_class _ (ExprCall fn' vs')) →
-    K' = comp_ectx K empty_ectx ∧ fn' = fn ∧ vs' = vs.
-  Proof.
-    intros HH. destruct (call_in_ctx _ _ _ _ _ HH) as [[K'' ->]|[? H2]].
-    { rewrite -fill_comp in HH. apply fill_inj in HH.
-      destruct (fill_class K'' (of_class _ (ExprCall fn' vs'))) as [Hc|Hc].
-      { rewrite -HH /= to_of_class //. }
-      2: { exfalso. rewrite /to_val to_of_class in Hc. by apply is_Some_None in Hc. }
-      subst K''. rewrite fill_empty in HH. apply of_class_inj in HH. by simplify_eq. }
-    { exfalso. apply of_class_inj in H2. congruence. }
-  Qed.
-  Lemma step_by_val p K' K_redex e1' e1_redex σ :
-      fill K' e1' = fill K_redex e1_redex →
-      to_val e1' = None →
-      is_head_redex p (e1_redex, σ) →
-      ∃ K'', K_redex = comp_ectx K' K''.
-  Proof.
-    rewrite /to_val => ? He1'. eapply step_by_val'; first done.
-    destruct (to_class e1') as [[]|]; done.
-  Qed.
-  Lemma head_ctx_step_val p K e σ:
-    is_head_redex p (fill K e, σ) → K = empty_ectx ∨ is_Some (to_val e).
-  Proof.
-    intros [?|[v Hv]]%head_ctx_step_val'; first by left. right.
-    rewrite /to_val Hv. eauto.
-  Qed.
-  Lemma call_head_step_inv p f vs σ X :
-    head_step p (of_class Λ (ExprCall f vs), σ) X →
-    (∀ fn e2, p !! f = Some fn → Some e2 = apply_func fn vs → X (e2, σ)).
-  Proof. eapply call_head_step. Qed.
-  Lemma call_head_step_intro p f vs fn σ er :
-    p !! f = Some fn →
-    Some er = apply_func fn vs →
-    head_step p (of_call Λ f vs, σ) (λ '(e', σ'), e' = er ∧ σ' = σ).
-  Proof.
-    intros ? ?. eapply call_head_step; intros; simplify_eq.
-    split; congruence.
-  Qed.
-
-  Lemma head_step_is_head_redex p x X : head_step p x X → is_head_redex p x.
-  Proof.
-    intros H. eapply umrel_upclosed; eauto.
-  Qed.
-
-  (* All non-value redexes are at the root.  In other words, all sub-redexes are
-     values. *)
-  Definition sub_redexes_are_values (e : expr Λ) :=
-    ∀ K e', e = fill K e' → to_val e' = None → K = empty_ectx.
-
-  Definition prim_step_mrel (p : prog Λ) : multirelation (expr Λ * state Λ) :=
-    λ '(e1, σ1) X,
-      ∃ K e1',
-        e1 = fill K e1' ∧
-        head_step p (e1', σ1) (λ '(e2', σ2), X (fill K e2', σ2)).
-
-  Program Definition prim_step (p : prog Λ) : umrel (expr Λ * state Λ) :=
-    {| mrel := prim_step_mrel p |}.
-  Next Obligation.
-    intros p [e1 σ1] *.
-    intros (K & e' & -> & Hstep) HH. do 2 eexists. split_and!; eauto.
-    eapply umrel_upclosed; eauto. intros [? ?]. eauto.
-  Qed.
-
-  Definition has_ub (p : prog Λ) (e : expr Λ) (σ : state Λ) :=
-    ∃ X, prim_step p (e, σ) X ∧ ∀ x, ¬ X x.
-
-  (** * Some lemmas about this language *)
-  Lemma to_of_val v : to_val (of_val Λ v) = Some v.
-  Proof. rewrite /to_val /of_val to_of_class //. Qed.
-  Lemma of_to_val e v : to_val e = Some v → of_val Λ v = e.
-  Proof.
-    rewrite /to_val /of_val => Hval. apply of_to_class.
-    destruct (to_class e) as [[]|]; simplify_option_eq; done.
-  Qed.
-  Lemma of_to_val_flip v e : of_val Λ v = e → to_val e = Some v.
-  Proof. intros <-. by rewrite to_of_val. Qed.
-  Lemma val_head_stuck p e σ X: head_step p (e, σ) X → to_val e = None.
-  Proof.
-    destruct (to_val e) as [v|] eqn:Hval; last done.
-    rewrite -(of_to_val e v) //. intros []%val_head_step.
-  Qed.
-  Lemma fill_val K e : is_Some (to_val (fill K e)) → is_Some (to_val e).
-  Proof.
-    intros Hval. destruct (fill_class K e) as [HK|He].
-    - apply is_val_is_class. done.
-    - subst K. move: Hval. rewrite fill_empty. done.
-    - done.
-  Qed.
-  Lemma val_stuck p e σ X: prim_step p (e, σ) X → to_val e = None.
-  Proof.
-    intros (K & e1' & -> & ?%val_head_stuck).
-    apply eq_None_not_Some. by intros ?%fill_val%eq_None_not_Some.
-  Qed.
-
-  Lemma to_of_call f vs : to_call (of_call Λ f vs) = Some (f, vs).
-  Proof. rewrite /to_call /of_call to_of_class //. Qed.
-  Lemma of_to_call e f vs : to_call e = Some (f, vs) → of_call Λ f vs = e.
-  Proof.
-    rewrite /to_call /of_call => Hval. apply of_to_class.
-    destruct (to_class e) as [[] | ]; simplify_option_eq; done.
-  Qed.
-  Lemma of_to_call_flip f vs e : of_call Λ f vs = e → to_call e = Some (f, vs).
-  Proof. intros <-. apply to_of_call. Qed.
-
-  Global Instance of_val_inj : Inj (=) (=) (of_val Λ).
-  Proof. by intros v v' Hv; apply (inj Some); rewrite -!to_of_val Hv. Qed.
-
-  Lemma extcall_ctx_has_ub p K f vs σ :
-    p !! f = None →
-    has_ub p (fill K (of_class Λ (ExprCall f vs))) σ.
-  Proof.
-    intros H.
-    exists (fun x => False).
-    split; last tauto.
-    econstructor. eexists; split; first done.
-    eapply call_head_step. intros ?? Hc _. rewrite H in Hc; congruence.
-  Qed.
-
-  Lemma fill_not_val K e : to_val e = None → to_val (fill K e) = None.
-  Proof. rewrite !eq_None_not_Some. eauto using fill_val. Qed.
-
-  Lemma head_prim_step p e1 σ1 X :
-    head_step p (e1, σ1) X → prim_step p (e1, σ1) X.
-  Proof.
-    intros Hstep. exists empty_ectx, e1. split.
-    - by rewrite fill_empty.
-    - intros *. eapply umrel_upclosed; eauto.
-      intros [? ?]. rewrite fill_empty //.
-  Qed.
-
-  Lemma fill_prim_step p K e1 σ1 X X' :
-    (∀ e2 σ2, X (e2, σ2) → X' (fill K e2, σ2)) →
-    prim_step p (e1, σ1) X →
-    prim_step p (fill K e1, σ1) X'.
-  Proof.
-    intros HX (K' & e1' & -> & Hstep). rewrite fill_comp /=.
-    do 2 eexists. split_and!; eauto.
-    eapply umrel_upclosed; eauto. intros [? ?].
-    rewrite -fill_comp. eauto.
-  Qed.
-  Lemma fill_prim_step' p K e1 σ1 X :
-    prim_step p (e1, σ1) X →
-    prim_step p (fill K e1, σ1)
-        (λ '(e2', σ2), ∃ e2, e2' = fill K e2 ∧ X (e2, σ2)).
-  Proof.
-    intros Hstep. eapply fill_prim_step with (X' := λ _, _) in Hstep.
-    - eapply Hstep.
-    - intros ? ? ?. simpl. eexists. eauto.
-  Qed.
-
-  Lemma prim_head_step p e σ X :
-    prim_step p (e, σ) X → sub_redexes_are_values e → head_step p (e, σ) X.
-  Proof.
-    intros (K & e1' & -> & Hstep) ?.
-    assert (K = empty_ectx) as -> by eauto 10 using val_head_stuck.
-    rewrite fill_empty. eapply umrel_upclosed; [apply Hstep|].
-    intros [? ?]. rewrite fill_empty //.
-  Qed.
-
-  Lemma head_reducible_prim_step_ctx p K e1 σ1 X :
-    is_head_redex p (e1, σ1) →
-    prim_step p (fill K e1, σ1) X →
-    head_step p (e1, σ1) (λ '(e2', σ2), ∀ e2, e2 = fill K e2' → X (e2, σ2)).
-  Proof.
-    intros HhstepK (K' & e1' & HKe1 & Hstep).
-    edestruct (step_by_val p K) as [K'' ?];
-      eauto using val_head_stuck; simplify_eq/=; first by eapply head_step_is_head_redex.
-    rewrite -fill_comp in HKe1; simplify_eq.
-    apply head_ctx_step_val in HhstepK as [?|[v ?]]; simplify_eq.
-    - rewrite fill_empty. eapply umrel_upclosed; [apply Hstep|].
-      intros [e σ]. rewrite -fill_comp fill_empty //. by intros ? ? ->.
-    - apply val_head_stuck in Hstep; simplify_eq.
-  Qed.
-
-  Lemma head_reducible_prim_step p e1 σ1 X :
-    is_head_redex p (e1, σ1) →
-    prim_step p (e1, σ1) X →
-    head_step p (e1, σ1) X.
-  Proof.
-    intros Hred Hpstep.
-    epose proof (head_reducible_prim_step_ctx _ empty_ectx _ _ X Hred) as Hhstep.
-    eapply umrel_upclosed.
-    - eapply Hhstep. by rewrite fill_empty.
-    - intros [e σ]. rewrite fill_empty. eauto.
-  Qed.
-
-  Lemma prim_step_call_inv p K f vs e' σ X :
-    prim_step p (fill K (of_call Λ f vs), σ) X →
-    ∀ er fn,
-      Some er = apply_func fn vs → p !! f = Some fn →
-      X (fill K er, σ).
-  Proof.
-    intros (K' & e1 & Hctx & Hstep) ?? Heq1 Heq2.
-    pose proof (head_step_is_head_redex _ _ _ Hstep) as Hredex.
-    eapply step_by_val in Hredex as H'; eauto; last apply to_val_of_call.
-    destruct H' as [K'' Hctx']; subst K'.
-    rewrite -fill_comp in Hctx. eapply fill_inj in Hctx.
-    destruct (fill_class K'' e1) as [->|Hval].
-    - apply is_call_is_class. erewrite of_to_call_flip; eauto.
-    - rewrite fill_empty in Hctx. subst e1.
-      eapply call_head_step_inv in Hstep. 2-3:done.
-      rewrite -fill_comp fill_empty// in Hstep.
-    - apply val_head_stuck in Hstep. apply not_eq_None_Some in Hval. done.
-  Qed.
-
   Lemma val_prim_step p v σ X :
-   ¬ prim_step p (of_val Λ v, σ) X.
-  Proof.
-    intros (K & e1' & Heq & Hstep').
-    edestruct (fill_val K e1') as (v1''& ?).
-    { rewrite -Heq. rewrite to_of_val. by exists v. }
-    eapply val_head_step.
-    erewrite <-(of_to_val e1') in Hstep'; eauto.
-  Qed. 
+    prim_step p (of_val Λ v, σ) X → False.
+  Proof. apply mlanguage_mixin. Qed.
+  Lemma call_prim_step p e f vs C σ X :
+      is_call e f vs C →
+        prim_step p (e, σ) X ↔
+        (∀ (fn : func Λ) e2,
+          p !! f = Some fn → Some e2 = apply_func fn vs → X (resume_with C e2, σ)).
+  Proof. apply mlanguage_mixin. Qed.
 
-  Lemma fill_step_inv p K e1' σ1 X :
-    to_val e1' = None →
-    prim_step p (fill K e1', σ1) X →
-    prim_step p (e1', σ1) (λ '(e2', σ2), X (fill K e2', σ2)).
+  Lemma not_is_call e : is_Some (to_val e) ↔ (∀ f vs C, ¬ is_call e f vs C).
+  Proof. apply mlanguage_mixin. Qed.
+
+  Lemma not_is_call_2 e f vs C : is_call e f vs C → to_val e = None.
   Proof.
-    intros ? (K'' & e'' & Heq & Hstep).
-    pose proof (head_step_is_head_redex _ _ _ Hstep) as Hredex.
-    eapply step_by_val in Hredex as Hstep'; eauto. destruct Hstep' as [K' ->].
-    rewrite -fill_comp in Heq. apply (inj (fill _)) in Heq as ->.
-    do 2 eexists; split_and!; eauto. clear Hredex.
-    eapply multirelations.umrel_upclosed; eauto. intros [? ?].
-    rewrite -fill_comp//.
+    intros H; destruct (to_val e) eqn:Heq; try done.
+    exfalso; apply mk_is_Some in Heq.
+    eapply not_is_call in Heq. done.
   Qed.
 
-  Lemma call_prim_step_fill p K f vs σ X :
-    prim_step p (fill K (of_class Λ (ExprCall f vs)), σ) X →
-    ∀ (fn : func Λ) e2,
-      p !! f = Some fn →
-      apply_func fn vs = Some e2 →
-      X (fill K e2, σ).
+  Lemma not_is_call_1 e v f vs C : to_val e = Some v → ¬ is_call e f vs C.
   Proof.
-    intros (K' & e1 & Hfill%eq_sym & Hstep) ?? HH1 HH2.
-    pose proof (call_in_ctx _ _ _ _ _ Hfill) as [[K'' ->]|[? Hval]].
-    { rewrite -fill_comp in Hfill. apply fill_inj in Hfill. subst e1.
-      pose proof (head_step_is_head_redex _ _ _ Hstep) as Hredex.
-      pose proof (head_ctx_step_val _ _ _ _ Hredex) as [->|[? Hval]].
-      { rewrite fill_empty in Hstep. eapply call_head_step in Hstep. 2-3:done.
-        rewrite -!fill_comp fill_empty//. }
-      { exfalso. rewrite /to_val to_of_class// in Hval. } }
-    { exfalso. subst. apply val_head_stuck in Hstep. rewrite /to_val to_of_class// in Hstep. }
-  Qed.
-
-  Lemma call_prim_step p f vs σ X :
-    prim_step p (of_class Λ (ExprCall f vs), σ) X →
-    ∀ (fn : func Λ) e2,
-      p !! f = Some fn →
-      apply_func fn vs = Some e2 →
-      X (e2, σ).
-  Proof.
-    intros H. epose proof (call_prim_step_fill p empty_ectx _ _ _ _) as Hp.
-    rewrite !fill_empty in Hp. intros fn e2 H1 H2. specialize (Hp H fn e2 H1).
-    rewrite fill_empty// in Hp. by eapply Hp.
+    intros H; revert f vs C; apply not_is_call. by eexists.
   Qed.
 
   (* There is no NB *)
   Lemma prim_step_is_total p e σ : to_val e = None → prim_step p (e,σ) (λ _, True).
-  Proof.
-    intros H.
-    induction e using (induction_ltof1 _ (expr_size)); unfold ltof in *.
-    destruct (head_redex_cases p e σ) as [(v&Hv)|[Hredex|(Hnredex&K&e'&->&He'&HK)]].
-    - congruence.
-    - eapply head_prim_step, Hredex.
-    - eapply fill_prim_step; last first; first eapply H0.
-      + by eapply fill_size.
-      + done.
-      + tauto.
-  Qed.
+  Proof. apply mlanguage_mixin. Qed.
 
   Class IntoVal (e : expr Λ) (v : val) :=
     into_val : of_val Λ v = e.
@@ -520,47 +138,6 @@ Section mlanguage.
     apply TCForall_Forall, Forall_fmap, Forall_true=> v.
     rewrite /AsVal /=; eauto.
   Qed.
-
-  Record pure_step p (e1 : expr Λ) (e2 : expr Λ) := {
-    pure_step_not_val : to_val e1 = None;
-    pure_step_det σ1 X :
-      prim_step p (e1, σ1) X → X (e2, σ1)
-  }.
-
-  Class PureExec (φ : Prop) (n : nat) p (e1 : expr Λ) (e2 : expr Λ) :=
-    pure_exec : φ → relations.nsteps (pure_step p) n e1 e2.
-
-  Lemma pure_exec_fill φ n p e1 e2 K :
-    PureExec φ n p e1 e2 →
-    PureExec φ n p (fill K e1) (fill K e2).
-  Proof.
-    intros H Hφ. specialize (H Hφ). induction H as [|n x y z [Hval Hdet] Hstep IH]; econstructor.
-    - econstructor.
-      + by eapply fill_not_val.
-      + intros σ1 X HH%fill_step_inv; last apply Hval.
-        apply Hdet in HH; eauto.
-    - apply IH.
-  Qed.
-
-  Lemma pure_step_ctx p K e1 e2 :
-    pure_step p e1 e2 →
-    pure_step p (fill K e1) (fill K e2).
-  Proof.
-    intros [Hred Hstep]. split.
-    - by eapply fill_not_val.
-    - intros σ1 X HstepK%fill_step_inv; last done.
-      apply Hstep in HstepK. eauto.
-  Qed.
-
-  Lemma pure_step_nsteps_ctx K n p e1 e2 :
-    relations.nsteps (pure_step p) n e1 e2 →
-    relations.nsteps (pure_step p) n (fill K e1) (fill K e2).
-  Proof. eauto using nsteps_congruence, pure_step_ctx. Qed.
-
-  Lemma pure_exec_ctx K P n p e1 e2 :
-    PureExec P n p e1 e2 →
-    PureExec P n p (fill K e1) (fill K e2).
-  Proof. rewrite /PureExec; eauto using pure_step_nsteps_ctx. Qed.
 
 End mlanguage.
 
